updating reconstruction

Smt/Reconstruction/Certifying/Util.lean
@@ -1,64 +1,87 @@
 import Lean
 
-open Lean.Expr Lean
+open Lean Expr Elab.Tactic Meta
 
-def andN : List Prop → Prop := λ l =>
-  match l with
-  | [] => True
-  | h :: [] => h
-  | h :: t  => h ∧ andN t
+def andN : List Prop → Prop
+| [] => True
+| h :: [] => h
+| h :: t  => h ∧ andN t
  
-def orN : List Prop → Prop := λ l =>
-  match l with
-  | [] => False
-  | h :: [] => h
-  | h₁ :: h₂ :: t  => h₁ ∨ orN (h₂ :: t)
+def orN : List Prop → Prop
+| [] => False
+| h :: [] => h
+| h₁ :: h₂ :: t  => h₁ ∨ orN (h₂ :: t)
  
-def notList : List Prop → List Prop :=
-  List.map Not
+def notList : List Prop → List Prop := List.map Not
 
 def notExpr : Expr → Expr
 | app (const `Not ..) e => e
 | e => mkApp (mkConst `Not) e
 
-def collectNOrNegArgs : Expr → Nat → List Expr
-| app (app (const `Or ..) e) _,  1       => [notExpr e]
-| app (app (const `Or ..) e1) e2, n + 1 => (notExpr e1) :: collectNOrNegArgs e2 n
+def collectOrNNegArgs : Expr → Nat → List Expr
+| app (app (const `Or ..) e) _,  1      => [notExpr e]
+| app (app (const `Or ..) e1) e2, n + 1 =>
+  notExpr e1 :: collectOrNNegArgs e2 n
 | e, _ => [e]
 
+-- Creates the expr corresponding to the list of values passed
+-- The second argument is the type of the elements of the list
 def listExpr : List Expr → Expr → Expr
-| [], ty => mkApp (const `List.nil [Level.zero]) ty
-| e::es, ty => mkApp (mkApp (mkApp (const `List.cons [Level.zero]) ty) e) (listExpr es ty)
+| [], ty    => mkApp (const `List.nil [Level.zero]) ty
+| e::es, ty =>
+  mkApp (mkApp (mkApp (const `List.cons [Level.zero]) ty) e) (listExpr es ty)
 
 def collectPropsInOrChain : Expr → List Expr
 | app (app (const `Or ..) e₁) e₂ => e₁ :: collectPropsInOrChain e₂
 | e => [e]
 
 def createOrChain : List Expr → Expr
-| [] => mkConst `unreachable
-| [h] => h
+| []   => panic! "createOrChain with empty list"
+| [h]  => h
 | h::t => app (app (mkConst `Or) h) $ createOrChain t
+
+def getIndex : Expr → Expr → Option Nat
+| t, app (app (const `Or ..) e1) e2 =>
+    if e1 == t then some 0
+    else (. + 1) <$> getIndex t e2
+| t, e => if e == t then some 0
+          else none
 
 def getCongAssoc' : Nat → Name → Term
 | 0,     n => mkIdent n
-| i + 1, n => Syntax.mkApp (mkIdent `congOrLeft) #[getCongAssoc' i n]
+| i + 1, n =>
+  Syntax.mkApp (mkIdent `congOrLeft) #[getCongAssoc' i n]
 
+-- tactics for parenthesizing the prefix of an or-chain
 def getCongAssoc : Nat → Name → List Term
 | 0,     _ => []
 | 1,     n => [getCongAssoc' 0 n]
 | i + 2, n => (getCongAssoc' (i + 1) n) :: (getCongAssoc (i + 1) n)
 
-def getLength (o : Expr) : Nat :=
-  match o with
-  | app (app (const `Or ..) _) e2 => 1 + getLength e2
-  | _ => 1
+def getLength : Expr → Nat
+| app (app (const `Or ..) _) e2 => 1 + getLength e2
+| _ => 1
 
 def getNatLit? : Expr → Option Nat
 | app (app _ (lit (Literal.natVal x))) _ => some x
 | _ => none
 
-open Lean.Elab.Tactic Lean.Meta in
+def getIthExpr? : Nat → Expr → Option Expr := λ i e =>
+  List.get? (collectPropsInOrChain e) i
+
+def stxToNat (h : Term) : TacticM Nat := do
+  let expr ← elabTerm h.raw none
+  match getNatLit? expr with
+  | some i => pure i
+  | none   => throwError "getNatLit? failed"
+
+def getTypeFromName (name : Name) : TacticM Expr :=
+  withMainContext do
+    let ctx ← getLCtx
+    inferType (ctx.findFromUserName? name).get!.toExpr
+
 def printGoal : TacticM Unit := do
   let currGoal ← getMainGoal
-  let currGoalType ← MVarId.getType currGoal
+  let currGoalType ← getMVarType currGoal
   logInfo m!"......new goal: {← instantiateMVars currGoalType}"
+
