Smt/Reconstruction/Certifying.lean
@@ -1,4 +1,8 @@
 import Smt.Reconstruction.Certifying.Boolean
+import Smt.Reconstruction.Certifying.Factor
+import Smt.Reconstruction.Certifying.LiftOrNToImp
 import Smt.Reconstruction.Certifying.PermutateOr
+import Smt.Reconstruction.Certifying.Pull
+import Smt.Reconstruction.Certifying.Quant
 import Smt.Reconstruction.Certifying.Resolution
 import Smt.Reconstruction.Certifying.Util
