Smt/Reconstruction/Certifying/Examples/ModusPonensExample/ModusPonens.lean
@@ -1,5 +1,5 @@
-import Smt.Reconstruction.Certifying.Boolean
-import Smt.Reconstruction.Certifying.Resolution
+import Meta.Boolean
+import Meta.Resolution
 
 theorem mpCvc5 (P Q : Prop) : ¬ (P → (P → Q) → Q) → False :=
   λ lean_a0 =>
@@ -7,7 +7,7 @@ theorem mpCvc5 (P Q : Prop) : ¬ (P → (P → Q) → Q) → False :=
     have lean_s1     := notImplies1 lean_s0
     have lean_s2     := impliesElim lean_s1
     have lean_s4     := notImplies1 lean_a0
-    have lean_s6     := by resolution_1 lean_s4, lean_s2, P
+    have lean_s6     := by R1 lean_s4, lean_s2, P
     have lean_s9     := notImplies2 lean_s0
     contradiction lean_s6 lean_s9
 
