Smt/Reconstruction/Certifying/Factor.lean
@@ -1,0 +1,77 @@
+import Lean
+
+import Smt.Reconstruction.Certifying.Boolean
+import Smt.Reconstruction.Certifying.Pull
+
+open Lean Elab.Tactic Meta
+
+def congDupOr (i : Nat) (nm : Ident) (last : Bool) : TacticM Syntax :=
+  match i with
+  | 0 =>
+    if last then `(dupOr₂ $nm)
+    else `(dupOr $nm)
+  | (i' + 1) => do
+    let nm' := mkIdent (Name.mkSimple "w")
+    let r ← congDupOr i' nm' last
+    let r: Term := ⟨r⟩
+    `(congOrLeft (fun $nm' => $r) $nm)
+
+-- i: the index fixed in the original list
+-- j: the index of li.head! in the original list
+def loop (i j n : Nat) (pivot : Expr) (li : List Expr) (nm : Ident) : TacticM Ident :=
+  match li with
+  | [] => return nm
+  | e::es =>
+    if e == pivot then do
+      -- step₁: move expr that is equal to the pivot to position i + 1
+      let step₁ ←
+        if j > i + 1 then
+          let fname ← mkIdent <$> mkFreshId
+          let e ← getTypeFromName nm.getId
+          let t ← instantiateMVars e
+          pullIndex2 (i + 1) j nm t fname
+          pure fname
+        else pure nm
+
+      -- step₂: apply congOrLeft i times with dupOr
+      let step₂: Ident ← do
+        let last := i + 1 == n - 1
+        let tactic ← congDupOr i step₁ last 
+        let tactic := ⟨tactic⟩
+        let fname ← mkIdent <$> mkFreshId
+        evalTactic (← `(tactic| have $fname := $tactic))
+        pure fname
+
+      loop i j (n - 1) pivot es step₂
+    else loop i (j + 1) n pivot es nm
+
+def factorCore (type : Expr) (source result : Ident) : TacticM Unit :=
+  withMainContext do
+    let mut li := collectPropsInOrChain type
+    let n := li.length
+    let mut answer := source
+    for i in List.range n do
+      li := List.drop i li
+      match li with
+      | [] => break
+      | e::es => do
+        answer ← loop i (i + 1) (li.length + i) e es answer
+        let e ← getTypeFromName answer.getId
+        let t ← instantiateMVars e
+        li := collectPropsInOrChain t
+    evalTactic (← `(tactic| have $result := $answer))
+
+syntax (name := factor) "factor" term "," ident : tactic
+
+@[tactic factor] def evalFactor : Tactic := fun stx =>
+  withMainContext do
+    let e ← elabTerm stx[1] none
+    let type ← inferType e
+    let source := ⟨stx[1]⟩
+    let result := ⟨stx[3]⟩
+    factorCore type source result
+
+example : A ∨ A ∨ A ∨ A ∨ B ∨ A ∨ B ∨ A ∨ C ∨ B ∨ C ∨ B ∨ A → True :=
+  by intro h
+     factor h, bla
+     exact True.intro
