Smt/Reconstruction/Certifying/LiftOrNToImp.lean
@@ -1,0 +1,49 @@
+import Lean
+
+import Smt.Reconstruction.Certifying.Boolean
+import Smt.Reconstruction.Certifying.Util
+
+open Lean Elab Tactic Meta Expr
+open List
+
+def getGroupOrPrefixGoal : Expr → Nat → Expr
+| e, n => let props := collectPropsInOrChain e
+          let left := createOrChain (take n props)
+          let right := createOrChain (drop n props)
+          app (app (mkConst `Or) left) right
+
+-- groups the given prefix of the given hypothesis (assuming it is an
+-- or-chain) and adds this as a new hypothesis with the given name
+def groupOrPrefixCore (hyp type : Expr) (prefLen : Nat) (name : Name)
+  : TacticM Unit := withMainContext do
+    let l := getLength type
+    if prefLen > 1 && prefLen < l then
+      let mvarId ← getMainGoal
+      Meta.withMVarContext mvarId do
+        let newTerm := getGroupOrPrefixGoal type prefLen
+        let p ← Meta.mkFreshExprMVar newTerm MetavarKind.syntheticOpaque name
+        let (_, mvarIdNew) ← Meta.intro1P $ ← Meta.assert mvarId name newTerm p
+        replaceMainGoal [p.mvarId!, mvarIdNew]
+      for t in reverse (getCongAssoc (prefLen - 1) `orAssocDir) do
+        evalTactic  (← `(tactic| apply $t))
+      Tactic.closeMainGoal hyp
+    else throwError
+           "[groupOrPrefix]: prefix length must be > 1 and < size of or-chain"
+
+syntax (name := liftOrNToImp) "liftOrNToImp" term "," term : tactic
+
+@[tactic liftOrNToImp] def evalLiftOrNToImp : Tactic :=
+  fun stx => withMainContext do
+    let prefLen ← stxToNat ⟨stx[3]⟩
+    let fname1 ← mkFreshId
+    let hyp ← Tactic.elabTerm stx[1] none
+    let type ← inferType hyp
+    groupOrPrefixCore hyp type prefLen fname1
+    let fname2 ← mkIdent <$> mkFreshId
+    evalTactic (← `(tactic| intros $fname2))
+    evalTactic (← `(tactic| apply orImplies₃ $(mkIdent fname1)))
+    let li := listExpr (collectOrNNegArgs type prefLen) (Expr.sort Level.zero)
+    withMainContext do
+      let ctx ← getLCtx
+      let hyp2 := (ctx.findFromUserName? fname2.getId).get!.toExpr
+      Tactic.closeMainGoal $ mkApp (mkApp (mkConst `deMorgan₂) li) hyp2
