Smt/Reconstruction/Certifying/PermutateOr.lean
@@ -1,56 +1,38 @@
-import Smt.Reconstruction.Certifying.Resolution
-
 import Lean
-open Lean
-open Lean.Elab.Tactic Lean.Syntax Lean.Elab Lean.Expr
-open Lean.Elab.Tactic
+
+import Smt.Reconstruction.Certifying.Pull
+import Smt.Reconstruction.Certifying.Util
+
+open Lean Elab Tactic
 
 -- TODO: find a way to remove '?' without breaking the parser
 syntax (name := permutateOr) "permutateOr" term "," ("[" term,* "]")? : tactic
 
 def parsePermuteOr : Syntax → TacticM (List Nat)
-  | `(tactic| permutateOr $_, [ $[$hs],* ]) => hs.toList.mapM stxToNat
-  | _                                      => throwError "ble"
-where
-  stxToNat (h : TSyntax `term) : TacticM Nat := do
-    let expr ← elabTerm h.raw none
-    match getNatLit? expr with
-    | some i => pure i
-    | none   => throwError "bla"
-
-def getIthExpr : Nat → Expr → Option Expr
-  | Nat.zero, app (app (const `Or ..) t₁) _ => some t₁
-  | Nat.zero, t                             => some t -- last element in or chain
-  | i + 1,    app (app (const `Or ..) _) t₂ => getIthExpr i t₂
-  | _, _                                    => none
+  | `(tactic| permutateOr $_, [ $[$hs],* ]) =>
+    hs.toList.mapM stxToNat
+  | _ =>
+    throwError "[permutateOr]: wrong usage"
 
 @[tactic permutateOr] def evalPermutateOr : Tactic :=
   fun stx => withMainContext do
     let hyp ← elabTerm stx[1] none
     let type ← Meta.inferType hyp
     let hs ← parsePermuteOr stx
-    let conclusion ← go hs.reverse type hyp
+    let conclusion ← go hs.reverse type hyp stx[1]
     Tactic.closeMainGoal conclusion
-where go : List Nat → Expr → Expr → TacticM Expr
-       | [], _, hyp => return hyp
-       | (i::is), type, hyp => do
+where go : List Nat → Expr → Expr → Syntax → TacticM Expr
+       | [], _, hyp, _ => return hyp
+       | (i::is), type, hyp, stx => do
          let fname ← mkIdent <$> mkFreshId
-         let fnameId := fname.getId
          let ithExpr ←
-           match getIthExpr i type with
+           match getIthExpr? i type with
            | some e => pure e
            | none   => throwError "invalid permutation"
-         logInfo m!"{ithExpr}"
-         reorderCore ithExpr hyp fnameId
+         let type ← instantiateMVars (← Meta.inferType hyp)
+         pullCore ithExpr type stx fname
          withMainContext do
            let ctx ← getLCtx
-           let hyp' := (ctx.findFromUserName? fnameId).get!.toExpr
-           go is type hyp'
-
-
-example : A ∨ B ∨ C ∨ D ∨ E → True := by
-  intro h
-  trivial
-  /- permutateOr h, [2, 1, 3, 4, 0] -/
-  /- trivial -/
+           let hyp' := (ctx.findFromUserName? fname.getId).get!.toExpr
+           go is type hyp' stx
 
