Smt/Reconstruction/Certifying/Pull.lean
@@ -1,0 +1,124 @@
+import Lean
+
+import Smt.Reconstruction.Certifying.Boolean
+import Smt.Reconstruction.Certifying.LiftOrNToImp
+
+open Lean Elab Tactic
+
+def applyList (l: List Term) (res: Term) : TacticM Term :=
+  match l with
+  | [] => return res
+  | t::ts =>
+    withMainContext do
+      let res' := Syntax.mkApp t #[res]
+      let fname ← mkIdent <$> mkFreshId
+      evalTactic (← `(tactic| have $fname := $res'))
+      applyList ts fname
+
+def mkAppList : List Term → Ident → Syntax
+| [], id => id
+| t::ts, id =>
+  let rest := mkAppList ts id
+  let rest := ⟨rest⟩
+  Syntax.mkApp t #[rest]
+
+def congTactics (tactics : List Term) (i : Nat) (id : Ident) (last : Bool) : TacticM Syntax :=
+  match i with
+  | 0 => do
+    if last then
+      let innerProof := mkAppList tactics id
+      let innerProof: Term := ⟨innerProof⟩
+      `($innerProof)
+    else
+      let id' := mkIdent (Name.mkSimple "w")
+      let innerProof := mkAppList tactics id'
+      let innerProof: Term := ⟨innerProof⟩
+      `(congOrRight (fun $id' => $innerProof) $id)
+  | (i' + 1) => do
+    let id' := mkIdent (Name.mkSimple "w")
+    let r ← congTactics tactics i' id' last
+    let r: Term := ⟨r⟩
+    `(congOrLeft (fun $id' => $r) $id)
+
+-- pull j-th term in the orchain to i-th position (we start counting indices at 0)
+-- TODO: clear intermediate steps
+def pullIndex2 (i j : Nat) (hyp : Syntax) (type : Expr) (id : Ident) : TacticM Unit :=
+  if i == j then do
+    let hyp: Term := ⟨hyp⟩
+    evalTactic (← `(tactic| have $id := $hyp))
+  else withMainContext do
+    let last := getLength type == j + 1
+    let step₁: Ident ← 
+      if last then pure ⟨hyp⟩
+      else do
+        let v := List.take (j - i) $ getCongAssoc j `orAssocDir
+        let res: Term := ⟨hyp⟩
+        let step₁: Term ← applyList v res
+        let step₁: Ident := ⟨step₁⟩ 
+        pure step₁ 
+
+    let step₂: Ident ←
+      if last then do
+        let tactics := List.take (j - 1 - i) $ getCongAssoc (j - 1) `orAssocDir
+        let step₂: Term ← applyList tactics step₁
+        let step₂: Ident := ⟨step₂⟩
+        pure step₂
+      else do
+        let tactics₂ := List.reverse $ getCongAssoc (j - i - 1) `orAssocDir
+        let wrappedTactics₂: Syntax ← congTactics tactics₂ i step₁ last
+        let wrappedTactics₂: Term := ⟨wrappedTactics₂⟩
+        let fname₂ ← mkIdent <$> mkFreshId
+        evalTactic (← `(tactic| have $fname₂ := $wrappedTactics₂))
+        pure fname₂
+    
+    let orComm: Term := ⟨mkIdent `orComm⟩
+    let wrappedTactics₃ ← congTactics [orComm] i step₂ last
+    let wrappedTactics₃ := ⟨wrappedTactics₃⟩
+    let step₃ ← mkIdent <$> mkFreshId
+    evalTactic (← `(tactic| have $step₃ := $wrappedTactics₃))
+
+    let step₄: Ident ←
+      if last then pure step₃ 
+      else do
+        let u := List.reverse $ List.take (j - i) $ getCongAssoc j `orAssocConv
+        let step₄: Term ← applyList u step₃
+        let step₄: Ident := ⟨step₄⟩
+        pure step₄
+
+    evalTactic (← `(tactic| have $id := $step₄))
+
+syntax (name := pull2) "pull2" term "," term "," term "," ident : tactic
+
+@[tactic pull2] def evalPull2 : Tactic := fun stx => withMainContext do
+  let i ← stxToNat ⟨stx[1]⟩ 
+  let j ← stxToNat ⟨stx[3]⟩
+  let id: Ident := ⟨stx[7]⟩
+  let e ← elabTerm stx[5] none
+  let t ← instantiateMVars (← Meta.inferType e)
+  pullIndex2 i j stx[5] t id
+
+def pullIndex (index : Nat) (hypS : Syntax) (type : Expr) (id : Ident) : TacticM Unit :=
+  pullIndex2 0 index hypS type id
+
+-- tries to find pivot in the tail of type, even if it has length > 1 (as an or-chain)
+-- pulls it to the beginning if found
+def pullTail (pivot hyp type : Expr) (id : Ident) : TacticM Unit := do
+  let props := collectPropsInOrChain type
+  let target := collectPropsInOrChain pivot
+  let restLength := props.length - target.length
+  let propsTail := List.drop restLength  props
+  if propsTail == target then
+    let fname ← mkFreshId
+    groupOrPrefixCore hyp type restLength fname
+    evalTactic (← `(tactic| have $id := orComm $(mkIdent fname)))
+  else throwError ("term not found: " ++ (toString pivot))
+
+-- insert pivot in the first position of the or-chain
+-- represented by hyp
+def pullCore (pivot type : Expr) (hypS : Syntax) (id : Ident) : TacticM Unit :=
+  match getIndex pivot type with
+  | some i => pullIndex i hypS type id
+  | none   => withMainContext do
+    let ctx ← getLCtx
+    let hyp := (ctx.findFromUserName? hypS.getId).get!.toExpr
+    pullTail pivot hyp type id
