Smt/Reconstruction/Certifying/Quant.lean
@@ -1,0 +1,21 @@
+universe u
+
+theorem instForAll {A : Type u} {f : A → Prop} {a : A} :
+  (forall a' : A, f a') → f a := by
+  intro h
+  exact h a
+
+theorem instEqual₁ {A : Type u} {P : A → Prop} {t : A} :
+  (forall x : A, x = t → P x) → P t := by
+  intro h
+  exact h t rfl
+
+theorem instEqual₂ {A : Type u} {P : A → Prop} {t : A} :
+  P t → (forall x : A, x = t → P x) := by
+  intros h x r
+  rewrite [r]
+  exact h
+
+theorem instEqual {A : Type u} {P : A → Prop} {t : A} :
+  (forall x : A, x = t → P x) ↔ P t := ⟨instEqual₁, instEqual₂⟩
+
