Smt/Reconstruction/Certifying/Resolution.lean
@@ -1,80 +1,8 @@
-import Smt.Reconstruction.Certifying.Boolean
-
 import Lean
 
-open Lean Lean.Elab Lean.Elab.Tactic Lean.Meta
-open List Expr
+import Smt.Reconstruction.Certifying.Pull
 
--- eliminates first occurence of `e` in `o`
-def eliminate (e o : Expr) : Expr :=
-  match o with
-  | app s@(app (const `Or ..) e1) e2 =>
-    if e1 == e then e2 else
-      if e2 == e then e1 else
-        app s (eliminate e e2)
-  | e => e
-
--- assuming `o` to be an OrChain, returns how many Props are
--- to the left of `t`
-def getIndex (t o : Expr) : Option Nat :=
-  match o with
-  | app (app (const `Or ..) e1) e2 => if e1 == t then some 0
-                                      else (. + 1) <$> getIndex t e2
-  | e => if e == t then some 0
-         else none
-
-def tacticsLastIndex (index : Nat) : List Term :=
-  (mkIdent `orComm) :: reverse (getCongAssoc (index - 1) `orAssocDir)
-
-def tacticsRegular (index : Nat) : List Term :=
-  let tactics₁ := getCongAssoc index `orAssocConv
-  let tactics₂ := [ Syntax.mkApp (mkIdent `congOrRight) #[mkIdent `orComm] ]
-  let tactics₃ := reverse $
-    map (λ e => Syntax.mkApp (mkIdent `congOrRight) #[e])
-      (getCongAssoc (index - 1) `orAssocDir)
-  let tactics₄ := reverse (getCongAssoc index `orAssocDir)
-  tactics₁ ++ tactics₂ ++ tactics₃ ++ tactics₄
-
--- defines the expr corresponding to the goal of reorder,
--- assuming we want to pull `t` in `o`
-def reorderGoal (t o : Expr) : Expr :=
-  match o with
-  | app (app (const `Or ..) _) _ => app (app (mkConst `Or) t) (eliminate t o)
-  -- if `o` is a single expression then we're assuming it is equals to `t`
-  -- useful for corner cases (resolution that results in empty clause)
-  | _ => t
-
--- TODO: write cores for every rule
-def reorderCore (pivot hyp : Expr) (name : Name) : TacticM Unit :=
-  withMainContext do
-    let type ← Meta.inferType hyp
-    let index' := getIndex pivot type
-    let index ←
-      match index' with
-      | some i => pure i
-      | none   => throwError "term not found"
-    let l := getLength type
-    let arr : List Term :=
-      if index = 0 then []
-      else if l = index + 1 then tacticsLastIndex index
-           else tacticsRegular index
-    let new_term := reorderGoal pivot type
-    let mvarId ← getMainGoal
-    Meta.withMVarContext mvarId do
-      let p ← Meta.mkFreshExprMVar new_term MetavarKind.syntheticOpaque name
-      let (_, mvarIdNew) ← Meta.intro1P $ ← Meta.assert mvarId name new_term p
-      replaceMainGoal [p.mvarId!, mvarIdNew]
-      for s in arr do
-        evalTactic (← `(tactic| apply $s))
-      Tactic.closeMainGoal hyp
-
-syntax (name := reorder) "reorder" term "," ident "," ident : tactic
-
-@[tactic reorder] def evalReorder : Tactic := fun stx => withMainContext do
-  let pivot ← elabTerm stx[1] none
-  let hyp ← elabTerm stx[3] none
-  let name := stx[5].getId
-  reorderCore pivot hyp name
+open Lean Elab.Tactic Meta
 
 theorem resolution_thm : ∀ {A B C : Prop}, (A ∨ B) → (¬ A ∨ C) → B ∨ C := by
   intros A B C h₁ h₂
@@ -96,69 +24,63 @@ theorem resolution_thm₃ : ∀ {A B: Prop}, (A ∨ B) → ¬ A → B := λ orab
 
 theorem resolution_thm₄ : ∀ {A : Prop}, A → ¬ A → False := λ a na => na a
 
-#check Ident
-
 def resolutionCore (firstHyp secondHyp : Ident) (pivotTerm : Term) : TacticM Unit := do
-  let fname1 ← mkIdent <$> mkFreshId
-  let fname2 ← mkIdent <$> mkFreshId
+  let fident1 ← mkIdent <$> mkFreshId
+  let fident2 ← mkIdent <$> mkFreshId
   let notPivot : Term := Syntax.mkApp (mkIdent `Not) #[pivotTerm]
-  evalTactic  (← `(tactic| reorder $pivotTerm, $firstHyp, $fname1))
-  evalTactic  (← `(tactic| reorder $notPivot, $secondHyp, $fname2))
-  -- I dont know why but the context doesn't automatically refresh to include the new hypothesis
-  -- thats why we have another `withMainContext` here
-  withMainContext do
-    /- let bla ← elabTerm fname1 none -/
-    /- let ble ← elabTerm fname2 none -/
-    let ctx ← getLCtx
-    let reordFirstHyp ← inferType (ctx.findFromUserName? fname1.getId).get!.toExpr
-    let reordSecondHyp ← inferType (ctx.findFromUserName? fname2.getId).get!.toExpr
-    let len₁ := getLength reordFirstHyp
-    let len₂ := getLength reordSecondHyp
+  let pivotExpr     ← elabTerm pivotTerm none
+  let notPivotExpr  ← elabTerm notPivot none
+  let firstHypType  ← inferType (← elabTerm firstHyp none)
+  let secondHypType ← inferType (← elabTerm secondHyp none)
 
-    let lenGoal ← getLength <$> getMainTarget
+  let lenGoal ← getLength <$> getMainTarget
+  pullCore pivotExpr    firstHypType  firstHyp  fident1
+  pullCore notPivotExpr secondHypType secondHyp fident2
 
-    -- TODO: understand why this if's is necessary
-    if lenGoal > 2 then
-      for s in getCongAssoc (len₁ - 2) `orAssocConv do
-        evalTactic (← `(tactic| apply $s))
-        logInfo m!"....apply {s}"
-        printGoal
+  let mut len₁ := getLength firstHypType
+  if Option.isNone (getIndex pivotExpr firstHypType) then
+    len₁ := len₁ - (getLength pivotExpr) + 1
 
-    if len₁ > 1 then
-      if len₂ > 1 then
-        /- Tactic.closeMainGoal (mkApp (mkApp (mkConst `resolution_thm) bla) ble) -/
-        evalTactic (← `(tactic| exact resolution_thm $fname1 $fname2))
-        logInfo m!"..close goal with resolution_thm"
-      else
-        /- Tactic.closeMainGoal (mkApp (mkApp (mkConst `resolution_thm₃) bla) ble) -/
-        evalTactic (← `(tactic| exact resolution_thm₃ $fname1 $fname2))
-        logInfo m!"..close goal with resolution_thm₃"
+  let len₂ := getLength secondHypType
+
+  if lenGoal > 2 then
+    for s in getCongAssoc (len₁ - 2) `orAssocConv do
+      evalTactic (← `(tactic| apply $s))
+      logInfo m!"....apply {s}"
+      printGoal
+
+  if len₁ > 1 then
+    if len₂ > 1 then
+      evalTactic (← `(tactic| exact resolution_thm $fident1 $fident2))
+      logInfo m!"..close goal with resolution_thm"
     else
-      if len₂ > 1 then
-        /- Tactic.closeMainGoal (mkApp (mkApp (mkConst `resolution_thm₂) bla) ble) -/
-        evalTactic (← `(tactic| exact resolution_thm₂ $fname1 $fname2))
-        logInfo m!"..close goal with resolution_thm₂"
-      else
-        /- Tactic.closeMainGoal (mkApp (mkApp (mkConst `resolution_thm₄) bla) ble) -/
-        evalTactic (← `(tactic| exact resolution_thm₄ $fname1 $fname2))
-        logInfo m!"..close goal with resolution_thm₄"
-  
+      evalTactic (← `(tactic| exact resolution_thm₃ $fident1 $fident2))
+      logInfo m!"..close goal with resolution_thm₃"
+  else
+    if len₂ > 1 then
+      evalTactic (← `(tactic| exact resolution_thm₂ $fident1 $fident2))
+      logInfo m!"..close goal with resolution_thm₂"
+    else
+      evalTactic (← `(tactic| exact resolution_thm₄ $fident1 $fident2))
+      logInfo m!"..close goal with resolution_thm₄"
 
-syntax (name := resolution_1) "resolution_1" ident "," ident "," term : tactic
-
+syntax (name := resolution_1) "R1" ident "," ident "," term : tactic
 @[tactic resolution_1] def evalResolution_1 : Tactic :=
   fun stx => withMainContext do
-    let firstHyp : Ident := ⟨ stx[1] ⟩
-    let secondHyp : Ident := ⟨ stx[3] ⟩
-    let pivotTerm : Term := ⟨ stx[5] ⟩
+    let firstHyp : Ident := ⟨stx[1]⟩
+    let secondHyp : Ident := ⟨stx[3]⟩
+    let pivotTerm : Term := ⟨stx[5]⟩
     resolutionCore firstHyp secondHyp pivotTerm
 
-syntax (name := resolution_2) "resolution_2" ident "," ident "," term : tactic
-
+syntax (name := resolution_2) "R2" ident "," ident "," term : tactic
 @[tactic resolution_2] def evalResolution_2 : Tactic :=
   fun stx => withMainContext do
-    let firstHyp : Ident := ⟨ stx[1] ⟩
-    let secondHyp : Ident := ⟨ stx[3] ⟩
-    let pivotTerm : Term := ⟨ stx[5] ⟩
+    let firstHyp : Ident := ⟨stx[1]⟩
+    let secondHyp : Ident := ⟨stx[3]⟩
+    let pivotTerm : Term := ⟨stx[5]⟩
     resolutionCore secondHyp firstHyp pivotTerm
+
+example : A ∨ B ∨ D ∨ (W ∨ Z) → E ∨ F ∨ G ∨ ¬ (W ∨ Z) → A ∨ B ∨ D ∨ E ∨ F ∨ G := by
+  intros h₁ h₂
+  R1 h₁, h₂, (W ∨ Z)
 
